Kami/Ex/ProcMemCorrect.v
@@ -17,7 +17,7 @@ Section ProcFour.
 
   Variables (fetch: AbsFetch addrSize iaddrSize instBytes dataBytes)
             (dec: AbsDec addrSize instBytes dataBytes rfIdx)
-            (exec: AbsExec iaddrSize instBytes dataBytes rfIdx)
+            (exec: AbsExec addrSize iaddrSize instBytes dataBytes rfIdx)
             (ammio: AbsMMIO addrSize).
 
   Variable predictNextPc: forall ty, fullType ty (SyntaxKind (Pc iaddrSize)) -> (* pc *)
