Kami/Ex/SCMMInl.v
@@ -13,7 +13,7 @@ Section Inlined.
 
   Variables (fetch: AbsFetch addrSize iaddrSize instBytes dataBytes)
             (dec: AbsDec addrSize instBytes dataBytes rfIdx)
-            (exec: AbsExec iaddrSize instBytes dataBytes rfIdx)
+            (exec: AbsExec addrSize iaddrSize instBytes dataBytes rfIdx)
             (ammio: AbsMMIO addrSize).
 
   Variable (procInit: ProcInit iaddrSize dataBytes rfIdx)
