Kami/Ex/SCMMInv.v
@@ -15,7 +15,7 @@ Section Invariants.
 
   Variables (fetch: AbsFetch addrSize iaddrSize instBytes dataBytes)
             (dec: AbsDec addrSize instBytes dataBytes rfIdx)
-            (exec: AbsExec iaddrSize instBytes dataBytes rfIdx)
+            (exec: AbsExec addrSize iaddrSize instBytes dataBytes rfIdx)
             (ammio: AbsMMIO addrSize).
 
   Definition PgmInitNotMMIO :=
